theories/Example.v
@@ -1,0 +1,96 @@
+From FSUB Require Import QCLibs.
+From FSUB Require Import FSub.
+From FSUB Require Import Decidable.
+From FSUB Require Import Generator.
+
+
+Eval cbv in (show (all top (all top
+                                (arrow (tvar 0) (arrow (tvar 1) (tvar 0)))))) .
+(** 
+    {∀Top . {∀Top . (<0> -> (<1> -> <0>))}}
+ *)
+Sample (gen_exact_term0
+          empty
+          (all top (all top (arrow (tvar 0) (arrow (tvar 1) (tvar 0)))))).
+
+(** Expected: 
+   (Λ Top. (Λ Top. (λ : <0>. (λ : <1>. [id 1]))))
+ *)
+
+(** 
+    (Λ Top. (Λ Top. (λ : <0>. (λ : <1>. [id 1]))))
+ *)
+
+Eval cbv in (show
+               (all top (arrow (tvar 0)
+                               (all top (arrow (tvar 0) (tvar 0)))))).
+
+Sample (gen_exact_term0
+          empty
+          (all top (arrow (tvar 0)
+                          (all top (arrow (tvar 0) (tvar 0)))))).
+(** 
+    (Mutant: Lift tvar when get_bound)
+
+    For type
+    {∀Top . (<0> -> {∀Top . (<0> -> <0>)})},
+
+    without lifting: 
+
+    [(Λ Top. (λ : <0>. (Λ Top. (λ : <0>. [id 0]))))]
+    [(Λ Top. (λ : <0>. (Λ Top. (λ : <0>. [id 1]))))]
+
+    Only 
+      [(Λ Top. (λ : <0>. (Λ Top. (λ : <0>. [id 0]))))]
+    is correct.
+ *)
+
+
+Sample (gen_exact_term0
+          empty
+          (all top (arrow (tvar 0)
+                          (all top (arrow (tvar 0) (tvar 1)))))).
+
+(**
+    Only 
+      [(Λ Top. (λ : <0>. (Λ Top. (λ : <0>. [id 1]))))]
+    is correct.
+ *)
+
+Eval cbv in (show (all top (arrow (arrow (tvar 0) (tvar 0))
+                                  (all top (arrow (tvar 0)
+                                                  (arrow (tvar 0) (tvar 0))))))).
+
+Sample (gen_exact_term0
+          empty
+          (all top (arrow ((arrow (tvar 0) (tvar 0)))
+                          (all top (arrow (tvar 0)
+                                          (arrow (tvar 1) (tvar 1))))))).
+(**
+   (Λ Top. (λ : (<0> -> <0>). (Λ Top. (λ : <0>. [id 1]))))
+
+   (Λ Top. (λ : (<0> -> <0>). (Λ Top. (λ : <0>. (λ : <1>. [id 0])))))     
+ *)
+
+
+
+Sample (gen_exact_tvar0
+          (ebound (ebound (ebound (ebound empty top) top) top) top)). 
+
+
+Sample (gen_exact_typ0
+          (ebound
+             (evar
+                (ebound
+                   (evar
+                      (ebound
+                         (evar
+                            empty
+                            (tvar 0))
+                         top)
+                      (tvar 1))
+                   top)
+                (tvar 0))
+             top)). 
+
+
