theories/Generator.v
@@ -1,6 +1,7 @@
 From FSUB Require Import QCLibs.
 From FSUB Require Import FSub.
 From FSUB Require Import Decidable.
+From FSUB Require Import Reduction.
 
 Fixpoint count_var (E : env) : nat :=
   match E with
@@ -9,39 +10,13 @@ Fixpoint count_var (E : env) : nat :=
   | ebound E _ => (count_var E)
   end.
 
-Definition gen_typ_from_env (E : env) : G (option typ) :=
-  match count_tvar E with
-  | O => ret None
-  | S n => n' <- choose(0, n);; ret (Some (tvar n'))
+Fixpoint tlift (T : typ) (m : nat) :=
+  match m with
+  | O => T
+  | S m => tlift (tshift 0 T) m
   end.
 
-Definition gen_base_typ (E : env) : G typ:=
-  oT <- gen_typ_from_env E;;
-  match oT with
-  | None => ret top
-  | Some T => elems [top ; T]
-  end.
-
-
-(** ** Type Generator *)
-Fixpoint gen_typ (n : nat) (E : env) : G typ :=
-  match n with
-  | O => gen_base_typ E
-  | S n =>
-      let gen_arrow :=
-        T1 <- gen_typ n E ;;
-        T2 <- gen_typ n (evar E T1) ;;
-        ret (arrow T1 T2) in
-      let gen_all :=
-        T1 <- gen_typ n E ;;
-        T2 <- gen_typ n (ebound E T1) ;;
-        ret (all T1 T2) in
-      oneOf [gen_arrow ; gen_all ; gen_base_typ E]
-  end.
-
-Sample (gen_typ 3 empty).
-
-(** Try to generate something, if it fails then use [top] *)
+(** ** Generate (Almost) SystemF *)
 Definition gen_top_comb (g : G (option typ)) : G (option typ) := 
   a <- g ;;
   match a with
@@ -49,139 +24,287 @@ Definition gen_top_comb (g : G (option typ)) : G (option typ) :=
   | None => returnGen (Some top)
   end.
 
+Definition gen_exact_tvar0' (E : env) : list (G typ) :=
+  match count_tvar E with
+  | O => []
+  | S n => [n' <- choose(0, n);; ret (tvar n')]
+  end.
+
+Definition gen_exact_tvar0 (E : env) : (G (option typ)) :=
+  oneOf_ (ret None) (map (fmap Some) (gen_exact_tvar0' E)).
+
+Fixpoint gen_exact_var0' (E : env) : list typ :=
+  match E with
+  | empty => []
+  | ebound E _ => map (tshift 0) (gen_exact_var0' E)
+  | evar E T => T :: (gen_exact_var0' E)
+  end.
+
+Definition gen_exact_from_var0' (E : env) : list (G typ) :=
+  map ret (gen_exact_var0' E).
+
+Definition gen_exact_from_var0 (E : env) : (G (option typ)) :=
+  oneOf_ (ret None) (map (fmap Some) (gen_exact_from_var0' E)).
+
+(* There must be another way to write this *)
+Definition gen_exact_typ0'  (E : env) : G typ :=
+  let gs' := map (fun g => T <- g;; returnGen (arrow T T))
+                (gen_exact_tvar0' E) in
+  let g'' := returnGen (all top (arrow (tvar 0) (tvar 0))) in
+  oneOf_ g'' (gs' ++ (gen_exact_from_var0' E)).
+
 (** There's no term of type [top]. Thus, [top] should only be generated 
     in parametric type lambda [all].
   *)   
-Fixpoint gen_concrete_typ (n : nat) (E : env) : G (option typ) :=
+
+Definition gen_exact_typ0 (E : env) : G (option typ) :=
+  fmap Some (gen_exact_typ0' E). 
+
+Fixpoint gen_exact_typ (n : nat) (E : env) : G (option typ) :=
   match n with
-  | O => gen_typ_from_env E
+  | O => gen_exact_typ0 E
   | S n =>
-      (** Chances are that there's is no enough [tvar] to generate [arrow].
-       *)
-      let gen_arrow :=
-        T1 <- gen_concrete_typ n E ;;
-        T2 <- gen_concrete_typ n (evar E T1) ;;
-        ret (arrow T1 T2) in
       let gen_all :=
-        T1 <- gen_top_comb (gen_concrete_typ n E) ;;
-        T2 <- gen_concrete_typ n (ebound E T1) ;;
+        T1 <- oneOf [ret top;   (* allow top in TVar *)
+                     gen_exact_typ (pred (pred n)) E] ;;
+        T2 <- gen_exact_typ n (ebound E T1) ;;
         ret (all T1 T2) in
-      backtrack [(1, gen_arrow) ; (2, gen_all) ; (1, gen_typ_from_env E)]
+      let gen_arrow :=
+        T1 <- oneOf_ (gen_exact_typ (pred (pred n)) E)
+                     ((gen_exact_typ (pred (pred n)) E)
+                        :: (map (fmap Some) (gen_exact_tvar0' E)));;
+        T2 <- gen_exact_typ n (evar E T1) ;;
+        ret (arrow T1 T2) in
+      (** use [backtrack] since [gen_arrow] could fail *)
+      backtrack [(5, gen_arrow) ; (5, gen_all) ; (1, gen_exact_typ0 E)]
   end.
 
-
-Fixpoint tlift (X : nat) (T : typ) {struct T} : typ :=
-  match T with
-  | tvar Y      => tvar (Y + X) (* tvar (if le_gt_dec X Y then 1 + Y else Y) *)
-  | top         => top
-  | arrow T1 T2 => arrow (tlift X T1) (tlift X T2)
-  | all T1 T2   => all (tlift X T1) (tlift (1 + X) T2)
-  end.
+Sample (gen_exact_typ 3 empty).
 
 Fixpoint get_bound_vars (T : typ) (n m : nat) (E : env) : list term :=
   match E with
   | empty => []
   | ebound E _ => get_bound_vars T n (S m) E
   | evar E T' => 
-      let T'' := tlift m T' in 
       let rst := get_bound_vars T (S n) m E in 
-      if T = T'' ? then (var n) :: rst else rst
+      if T = (tlift T' m) ? then (var n) :: rst else rst
   end.
+
+Definition gen_bound_vars' (T : typ) (E : env) : list (G term) :=
+  map ret (get_bound_vars T 0 0 E).
 
 Definition gen_bound_vars (T : typ) (E : env) : G (option term) :=
   elems_ None (map Some (get_bound_vars T 0 0 E)).
 
-
-Fixpoint gen_concrete_base_typ (E : env) (T : typ) : G (option term) :=
-  let g : G (option term) :=
+(* FIXME : When meet [tvar n], resolve the type recursively *)
+Fixpoint gen_exact_term0 (E : env) (T : typ) : G (option term) :=
+  let g : (G (option term)) :=
     match T with
     | arrow T1 T2 =>
-        liftM (abs T1) (gen_concrete_base_typ (evar E T1) T2)
+        liftM (abs T1) (gen_exact_term0 (evar E T1) T2)
     | all T1 T2 =>
         liftM (tabs T1)
-              (gen_concrete_base_typ (ebound E T1) T2)
+              (gen_exact_term0 (ebound E T1) T2)
     | _ => ret None
     end
   in     
-  backtrack [ (1, gen_bound_vars T E) ;
-              (1, g) ].
+  backtrack [(1, g); (1, (gen_bound_vars T E))].
 
+Fixpoint gen_ftvar0 (n : nat) (E : env) (acc : list typ) : list typ :=
+  match E with
+  | empty => acc
+  | evar E _ => gen_ftvar0 n E acc
+  | ebound E _ => gen_ftvar0 (S n) E ((tvar n) :: acc)
+  end.
 
-Compute (show (all top (all top
-                            (arrow (tvar 0) (arrow (tvar 1) (tvar 0)))))) .
-(** 
-    {∀Top . {∀Top . (<0> -> (<1> -> <0>))}}
- *)
-Sample (gen_concrete_base_typ
-          empty
-          (all top (all top (arrow (tvar 0) (arrow (tvar 1) (tvar 0)))))).
+Definition gen_ftvar (E : env) : G (option typ) :=
+  elems_ None (map Some (gen_ftvar0 0 E [])).
 
-(** Expected: 
-   (Λ Top. (Λ Top. (λ : <0>. (λ : <1>. [id 1]))))
- *)
-
-(** 
-    (Λ Top. (Λ Top. (λ : <0>. (λ : <1>. [id 1]))))
- *)
-
-Compute (show
-        (all top (arrow (tvar 0)
-                          (all top (arrow (tvar 0) (tvar 0)))))).
-
-Sample (gen_concrete_base_typ
-          empty
-          (all top (arrow (tvar 0)
-                          (all top (arrow (tvar 0) (tvar 0)))))).
-(** 
-    (Mutant: Lift tvar when get_bound)
-
-    For type
-    {∀Top . (<0> -> {∀Top . (<0> -> <0>)})},
-
-    without lifting: 
-
-    [(Λ Top. (λ : <0>. (Λ Top. (λ : <0>. [id 0]))))]
-    [(Λ Top. (λ : <0>. (Λ Top. (λ : <0>. [id 1]))))]
-
-    Only 
-      [(Λ Top. (λ : <0>. (Λ Top. (λ : <0>. [id 0]))))]
-    is correct.
- *)
-
-
-Sample (gen_concrete_base_typ
-          empty
-          (all top (arrow (tvar 0)
-                          (all top (arrow (tvar 0) (tvar 1)))))).
-
-(**
-    Only 
-      [(Λ Top. (λ : <0>. (Λ Top. (λ : <0>. [id 1]))))]
-    is correct.
- *)
-
-Compute (show (all top (arrow (arrow (tvar 0) (tvar 0))
-                              (all top (arrow (tvar 0)
-                                              (arrow (tvar 0) (tvar 0))))))).
-
-Sample (gen_concrete_base_typ
-          empty
-          (all top (arrow ((arrow (tvar 0) (tvar 0)))
-                          (all top (arrow (tvar 0)
-                                          (arrow (tvar 1) (tvar 1))))))).
-(**
-   (Λ Top. (λ : (<0> -> <0>). (Λ Top. (λ : <0>. [id 1]))))
-
-   (Λ Top. (λ : (<0> -> <0>). (Λ Top. (λ : <0>. (λ : <1>. [id 0])))))     
-*)
-
-(** Generate terms from concrete types *)
-Fixpoint gen_concrete_term (n : nat) (E : env) (T : typ) :  :=
+(** Generate terms from exact types *)
+Fixpoint gen_exact_term (n : nat) (E : env) (T : typ) : G (option term) :=
   match n with
-  | O => gen_concrete_base_typ
+  | O => gen_exact_term0 E T
   | S n =>
-      match T with
-      | tvar n => gen_bound_vars
-      
-Fixpoint gen_sup_typ (fuel : nat) (E : env) (T : typ) : G typ :=
+      let g0 := gen_exact_term0 E T in
+      let g1 := 
+        match T with
+        | arrow T1 T2 =>
+            liftM (fun t2 => (abs T1 t2))
+                  (gen_exact_term n (evar E T1) T2)
+        | all T1 T2 => 
+            liftM (fun t2 => (tabs T1 t2))
+                  (gen_exact_term n (ebound E T1) T2)
+        | _ => returnGen None
+        end in
+      (** Generate App *)
+      let g2 :=
+        T1 <- gen_exact_typ (pred n) E;; (* include more context aware generation? *)
+        (* t1 <- gen_exact_term n (evar E T1) T;; *)
+        t1 <- gen_exact_term (pred n) E (arrow T1 T);;
+        t2 <- gen_exact_term n E T1;;
+        (* returnGen (Some (app (abs T1 t1) t2)) *)
+        returnGen (Some (app t1 t2))
+      in
+      (** Generate TApp *)
+      let g3 :=
+        T1 <- gen_exact_typ (pred n) E;; 
+        t1 <- gen_exact_term n E (all T1 (tshift 0 T));;
+        returnGen (Some (tapp t1 T1))
+      in backtrack [(1, g0); (1, g1); (1, g2); (1, g3)]
+  end
+.      
 
+Definition gen_exact (n : nat) : G (option term) :=
+  T <- gen_exact_typ n empty;;
+  gen_exact_term n empty T.
+
+Sample (gen_exact 5).
+
+Definition type_check' :=
+  fun E t T => type_check E t T 100. 
+Definition get_typ' :=
+  fun E t => get_typ E t 100. 
+
+(** ** Generate Subtype *)
+Definition sub_check' :=
+  fun e T1 T2 => sub_check e T1 T2 20. 
+
+(* TODO : Abstraction *)
+Definition gen_sub_tvar' (E : env) (T2 : typ) : list typ :=
+  let n := count_tvar E in
+  let fix f n1 :=
+    match n1 with
+    | O => []
+    | S n1 => 
+        match get_bound E n1 with
+        | None => []
+        | Some T1 => 
+            let T' := match sub_check' E T1 T2 with
+                      | Result true => [T1]
+                      | _ => []
+                      end in
+            T' ++ (f n1)
+        end
+    end in
+  f n.
+
+
+Definition gen_sub_tvar (E : env) (T2 : typ) : G typ :=
+  elems_ T2 (gen_sub_tvar' E T2). 
+
+Definition gen_sup_tvar' (E : env) (n1 : nat) : list typ :=
+  match get_bound E n1 with
+  | None => []
+  | Some T1 => 
+      let n := count_tvar E in
+      let fix f n2 :=
+        match n2 with
+        | O => []
+        | S n2 => 
+            match get_bound E n2 with
+            | None => []
+            | Some T2 => 
+                let T' := match sub_check' E T1 T2 with
+                          | Result true => [tvar n1]
+                          | _ => []
+                          end in
+                T' ++ (f n2)
+            end
+        end in
+      f n
+  end.
+
+
+Definition gen_sup_tvar (E : env) (n1 : nat) : G typ :=
+  elems_ (tvar n1) (gen_sup_tvar' E n1). 
+
+Fixpoint gen_sub_typ (n : nat) (E : env) (T : typ) : G typ :=
+  match n with
+  | O => ret T                  (** [sub] is reflexive *)
+  | S n =>
+      let g1 :=
+        match T with
+        | top =>
+            (** any <: [top] *)
+            T1 <- gen_exact_typ n E ;;
+            match T1 with
+            | Some T1 => ret T1
+            | None => ret top
+            end
+        | tvar n => ret (tvar n)
+        | arrow T1 T2 =>
+            (** [S1] :> [T1] -> 
+              [S2] <: [T2] ->
+              arrow [S1] [S2] <: arrow [T1] [T2] 
+             *)
+            S1 <- gen_sup_typ n E T1;;
+            S2 <- gen_sub_typ n E T2;;
+            ret (arrow S1 S2)
+        | all T1 T2 =>
+            S1 <- gen_sup_typ n E T1;;
+            S2 <- gen_sub_typ n (ebound E T1) T2;;
+            ret (all S1 S2)
+        end in
+      let g2 := map ret (gen_sub_tvar' E T) in
+      oneOf_ (ret T) ((ret T) :: g1 :: g2)
+  end
+with
+gen_sup_typ (n : nat) (E : env) (T : typ) : G typ :=
+  match n with
+  | O => ret T                  (** [sup] is reflexive *)
+  | S n =>
+      let g1 :=
+        match T with
+        | top => ret top        (** [top] is the top *)
+        | tvar n => gen_sup_tvar E n
+        | arrow T1 T2 =>
+            S1 <- gen_sub_typ n E T1;;
+            S2 <- gen_sup_typ n E T2;;
+            ret (arrow S1 S2)
+        | all T1 T2 =>
+            S1 <- gen_sub_typ n E T1;;
+            S2 <- gen_sup_typ n (ebound E T1) T2;;
+            ret (all S1 S2)
+        end in
+      oneOf [ret T ; g1]
+  end
+.
+
+(** ** Generate SystemF Sub *)
+(** Idea0: Fixpoint iteration *)
+
+Fixpoint multistep {A}
+           (n : nat)
+           (step : A -> option A)
+           (t : A)
+           (is_value : A -> bool) : @result (bool * A) :=
+  match n with
+  | O => OutOfFuel
+  | S n =>
+      match step t with
+      | Some t => multistep n step t is_value
+      | None => Result ((is_value t), t)
+      end
+  end.
+
+(** ** [C7] Weak Progress *)
+Definition prop_gen_progress :=
+  let fuel_type := 6 in
+  forAllMaybe (gen_exact_typ fuel_type empty) (fun T =>
+  forAllMaybe (gen_exact_term fuel_type empty T) (fun t =>
+  forAll (gen_sup_typ fuel_type empty T) (fun R =>
+  whenFail ("Gened Typ [T] is " ++ show T ++ nl ++ 
+            "Gened Sup [R] is " ++ show R ++ nl ++ 
+            "Gened Term [t] is " ++ show t ++ nl)
+           (((type_check' empty t T) = (Result true) ?) &&
+              (match multistep 40 step t dc_value with
+               | Result (true, t) => ((type_check' empty t T) = (Result true) ?)
+               | _ => false
+               end))%bool))).
+
+QuickChick prop_gen_progress.
+
+(** TODO : More Type-Parameter-Aware Term Generation
+    
+    Λ<:top. λ<:<0>. <: (<0> -> <0>). λ <:<0>. [0] [1]
+ *)
