theories/Properties.v
@@ -5,31 +5,96 @@ From FSUB Require Import Generator.
 From FSUB Require Import Reduction.
 
 
-Definition sub_check_100 (e : env) (T1 T2 : typ) : bool :=
-  match sub_check e T1 T2 100 with
-  | Result true => true
-  | _ => false
-  end.
+Definition type_check' :=
+  fun E t T => type_check E t T 100. 
+Definition get_typ' :=
+  fun E t => get_typ E t 100. 
 
-Definition prop_gen_wt :=
-  let fuel_type := 4 in
-  let fuel_expr := 4 in
-  forAll (gen_typ fuel_type) (fun T =>
-  forAllMaybe (gen_expr fuel_expr [] T) (fun t => 
-  whenFail ("Type was " ++ show T ++ nl ++ 
-            "Term was " ++ show t ++ nl ++
-            "With Type" ++ show (typeOf [] t) ++))
-           (typeOf [] t = Some T ?)).
-
-(** ** [C1] generated concrete [typ]s are well-formed *)
-Definition prop_gen_concrete_typ_wf :=
-  forAllMaybe (gen_concrete_typ 5 empty) (fun T =>
+(** ** [C1] generated exact [typ]s are well-formed *)
+Definition prop_gen_exact_typ_wf :=
+  forAllMaybe (gen_exact_typ 5 empty) (fun T =>
   whenFail ("Type is: " ++ show T ++ nl)
            (dc_wf_typ empty T)).
 
-QuickChick prop_gen_concrete_typ_wf.
+QuickChick prop_gen_exact_typ_wf.
 
-Locate "elems".
 
-Check (Some var).
+(** ** [C2-0] generated exact [term]s (base case) are well-typed *)
+Definition prop_gen_exact0_wt :=
+  let fuel_type := 4 in
+  let fuel_expr := 4 in
+  forAllMaybe (gen_exact_typ fuel_type empty) (fun T =>
+  forAllMaybe (gen_exact_term0 empty T) (fun t => 
+  whenFail ("Gened Type is" ++ show T ++ nl ++ 
+            "Gened Term is" ++ show t ++ nl ++
+            "Checked Type is" ++ show_result' (get_typ' empty t)
+           )
+           ((type_check' empty t T) = (Result true) ?))).
+
+QuickChick prop_gen_exact0_wt.
+
+(** ** [C2] generated exact [term]s are well-typed *)
+Definition prop_gen_exact_wt :=
+  let fuel_type := 6 in
+  let fuel_expr := 6 in
+  forAllMaybe (gen_exact_typ fuel_type empty) (fun T =>
+  forAllMaybe (gen_exact_term fuel_expr empty T) (fun t => 
+  whenFail ("Gened Type is" ++ show T ++ nl ++ 
+            "Gened Term is" ++ show t ++ nl ++
+            "Type of Term is" ++ show_result' (get_typ' empty t)
+           )
+           ((type_check' empty t T) = (Result true) ?))).
+
+
+QuickChick prop_gen_exact_wt.
+
+
+
+(** ** [C3] generated subtype [term]s are well-formed *)
+Definition prop_gen_sub_typ_wf :=
+  let fuel_type := 6 in
+  forAllMaybe (gen_exact_typ fuel_type empty) (fun T =>
+  forAll (gen_sub_typ fuel_type empty T) (fun S =>
+  whenFail ("Gened Type is" ++ show T ++ nl ++ 
+            "Gened SubT is" ++ show S ++ nl)
+           (dc_wf_typ empty T))).
+
+QuickChick prop_gen_sub_typ_wf.
+
+
+(** ** [C4] generated sub [typ]s are subtypes *)
+Definition prop_gen_sub_typ_sub :=
+  let fuel_type := 5 in
+  forAllMaybe (gen_exact_typ fuel_type empty) (fun T =>
+  forAll (gen_sub_typ fuel_type empty T) (fun S =>
+  whenFail ("Gened Type is" ++ show T ++ nl ++ 
+            "Gened SubT is" ++ show S ++ nl)
+           ((sub_check' empty S T) = (Result true) ?))).
+
+QuickChick prop_gen_sub_typ_sub.
+
+(** ** [C5] generated super [typ]s are super types *)
+Definition prop_gen_sup_typ_sup :=
+  let fuel_type := 5 in
+  forAllMaybe (gen_exact_typ fuel_type empty) (fun T =>
+  forAll (gen_sup_typ fuel_type empty T) (fun S =>
+  whenFail ("Gened Type is" ++ show T ++ nl ++ 
+            "Gened SupT is" ++ show S ++ nl)
+           ((sub_check' empty T S) = (Result true) ?))).
+
+QuickChick prop_gen_sup_typ_sup.
+
+(** ** [C6] Subtype Transitivity  *)
+Definition prop_gen_sub_trans :=
+  let fuel_type := 6 in
+  forAllMaybe (gen_exact_typ fuel_type empty) (fun T =>
+  forAll (gen_sub_typ fuel_type empty T) (fun S =>
+  forAll (gen_sub_typ fuel_type empty S) (fun R =>
+  whenFail ("Gened Typ [T] is " ++ show T ++ nl ++ 
+            "Gened Sub [S] is " ++ show S ++ nl ++ 
+            "Gened Sub [R] is " ++ show R ++ nl)
+           ((((sub_check' empty R S) = (Result true) ?)
+             && ((sub_check' empty S T) = (Result true) ?))%bool)))).
+
+QuickChick prop_gen_sub_trans.
 
